MathematicalLogic/Notation.lean
@@ -1,0 +1,37 @@
+import Mathlib.Order.BoundedOrder
+import Mathlib.Data.Vector
+
+universe u
+
+notation "[]ᵥ" => Vector.nil
+infixr:67 "∷ᵥ" => Vector.cons
+
+@[notation_class] class NotSymbol (α : Type u) where
+  not : α → α
+
+@[notation_class] class AndSymbol (α : Type u) where
+  and : α → α → α
+
+@[notation_class] class OrSymbol (α : Type u) where
+  or : α → α → α
+
+@[notation_class] class ImpSymbol (α : Type u) where
+  imp : α → α → α
+
+@[notation_class] class IffSymbol (α : Type u) where
+  iff : α → α → α
+
+@[notation_class] class ForallSymbol (α : Type u) where
+  all : α → α
+
+@[notation_class] class ExistsSymbol (α : Type u) where
+  exist : α → α
+
+prefix:58 "~ " => NotSymbol.not
+infix:56 " ⋁ " => OrSymbol.or
+infix:57 " ⋀ " => AndSymbol.and
+infixr:55 " ⟶ " => ImpSymbol.imp
+infix:55 " ⟷ " => IffSymbol.iff
+prefix:59 "∀' " => ForallSymbol.all
+prefix:59 "∃' " => ExistsSymbol.exist
+attribute [match_pattern] NotSymbol.not OrSymbol.or AndSymbol.and ImpSymbol.imp IffSymbol.iff ForallSymbol.all ExistsSymbol.exist
